{
 "cells": [
  {
   "cell_type": "markdown",
   "id": "75fafff4",
   "metadata": {},
   "source": [
    "# 18.06 Problem Set 10 Solutions"
   ]
  },
  {
   "cell_type": "markdown",
   "id": "33675fdf",
   "metadata": {},
   "source": [
    "## Problem 1 (5+5+5+5)\n",
    "\n",
    "In the [18.06 ODE lecture](https://nbviewer.org/github/mitmath/1806/blob/master/notes/ODEs.ipynb), we found that the position ($x$) and velocity ($v$) of a mass bouncing on a spring without friction are described by the equations:\n",
    "\n",
    "$$\n",
    "\\frac{d}{dt} \\underbrace{\\begin{pmatrix} x \\\\ v \\end{pmatrix}}_\\vec{x} =\n",
    "\\underbrace{\\begin{pmatrix} 0 & 1 \\\\ -k/m & 0 \\end{pmatrix}}_A \\vec{x}\n",
    "$$\n",
    "\n",
    "for (real) spring constant $k > 0$ and mass $m > 0$.\n",
    "\n",
    "**(a)** Show that by simply *rescaling* the variables $\\vec{x} = (x,v)$ to new variables $\\vec{y} = (a,b) = D \\vec{x}$ for some *diagonal* matrix $D$, then you can get equations:\n",
    "$$\n",
    "\\frac{d\\vec{y}}{dt} = B \\vec{y}\n",
    "$$\n",
    "where $B$ is (real) *anti-Hermitian* (also called *skew-Hermitian*): $B^H = -B$.  (What is the formula relating $B$ and $A$ via $D$?  $B$ and $A$ are \\_\\_\\_\\_\\_\\_ to one another.)\n",
    "\n",
    "**(b)** For *any* anti-Hermitian $B = -B^H$, the matrix $iB$ is a \\_\\_\\_\\_\\_\\_\\_\\_ matrix because $(iB)^H = \\_\\_\\_$.   It follows that the eigenvalues of $B$ are purely \\_\\_\\_\\_\\_\\_\\_\\_ and hence the solutions $\\vec{y}(t)$ of $d\\vec{y}/dt = B \\vec{y}$ are \\_\\_\\_\\_\\_\\_\\_\\_ (oscillating/growing/decaying).\n",
    "\n",
    "**(c)** For *any* anti-Hermitian $B = -B^H$, the matrix $Q = e^{Bt}$ is *unitary* (for any real $t$) because \\_\\_\\_\\_\\_\\_\\_\\_.  (Note: from the series definition of $e^A$, you can immediately see that $(e^A)^H = e^{A^H}$.)\n",
    "\n",
    "**(d)** Recall from class that $\\Vert Q \\vec{y} \\Vert = \\Vert \\vec{y} \\Vert$ for any unitary $Q$ (or more generally any $Q$ with orthonormal columns).   From this, derive that the solution $$\\vec{y}(t) = e^{Bt} \\vec{y}(0)$$ for your $B$ from part (a) *conserves energy*: $\\frac{1}{2} mv^2 + \\frac{1}{2} kx^2$ (kinetic + potential energy) is a *constant* as a function of time $t$."
   ]
  },
  {
   "cell_type": "markdown",
   "id": "e8b1c736",
   "metadata": {},
   "source": [
    "### Solution\n",
    "\n",
    "**(a)** By rescaling $\\vec{x} = (x,v)$ to new variables $\\vec{y} = (a,b) = D \\vec{x}$ for some diagonal matrix $D = \\begin{pmatrix} \\alpha & 0 \\\\ 0 & \\beta \\end{pmatrix}$, we have\n",
    "$$\n",
    "\\frac{d\\vec{y}}{dt} = \\frac{d (D\\vec{x})}{dt}= D\\frac{d \\vec{x}}{dt}  =\n",
    "DA \\vec{x} = DA D^{-1} \\vec{y} = \\begin{pmatrix} \\alpha & 0 \\\\ 0 & \\beta \\end{pmatrix} \\begin{pmatrix} 0 & 1 \\\\ -k/m & 0 \\end{pmatrix} \\begin{pmatrix} 1/\\alpha & 0 \\\\ 0 & 1/\\beta \\end{pmatrix} \\vec{y} = \\begin{pmatrix} 0 & \\frac{\\alpha}{\\beta} \\\\ -\\frac{\\beta k}{\\alpha m} & 0 \\end{pmatrix} \\vec{y} = B \\vec{y}.\n",
    "$$\n",
    "Now, \n",
    "$$\n",
    "B^H = \\begin{pmatrix} 0 & \\frac{\\alpha}{\\beta} \\\\ -\\frac{\\beta k}{\\alpha m} & 0 \\end{pmatrix}^H = \\begin{pmatrix} 0 & -\\frac{\\bar{\\beta} k}{\\bar{\\alpha} m} \\\\  \\frac{\\bar{\\alpha}}{\\bar{\\beta}} & 0 \\end{pmatrix}.\n",
    "$$\n",
    "For $B$ to be anti-Hermitian, i.e. $B = -B^H$, we have \n",
    "$$\n",
    "\\frac{\\alpha}{\\beta} = \\frac{\\bar{\\beta} k}{\\bar{\\alpha} m} \\Longleftrightarrow \\alpha^2 m = \\beta^2 k.\n",
    "$$\n",
    "Therefore, by taking $\\boxed{D = \\begin{pmatrix} \\sqrt{k} & 0 \\\\ 0 & \\sqrt{m} \\end{pmatrix}}$, we obtain an anti-Hermitian matrix $\\boxed{B = \\begin{pmatrix} 0 & \\sqrt{\\frac{k}{m}} \\\\ -\\sqrt{\\frac{k}{m}} & 0 \\end{pmatrix}}$.\n",
    "\n",
    "Note that the formula relating $B$ and $A$ is $\\boxed{B = D A D^{-1}}$, and hence $B$ and $A$ are **similar** to one another.\n",
    "\n",
    "\n",
    "**(b)** For any anti-Hermitian $B = -B^H$, the matrix $iB$ is a **Hermitian** matrix because $(iB)^H = \\boxed{-i B^H = -i(-B) = iB}$. \n",
    "\n",
    "By the property of Hermitian matrices, the eigenvalues of $iB$ are real. It follows that the eigenvalues of $B$ are purely **imaginary** and hence the solutions $\\vec{y}(t)$ of $d\\vec{y}/dt = B \\vec{y}$ are **oscillating**.\n",
    "\n",
    "**(c)** For any anti-Hermitian $B = -B^H$, we have \n",
    "$$\\boxed{QQ^H = e^{Bt} (e^{Bt})^{H} = e^{Bt} e^{(Bt)^H} = e^{Bt} e^{-Bt} =  e^{(B-B)t} = I}.$$\n",
    "Note that the second last equality above follows from the fact that $Bt$ and $-Bt$ commute. Therefore, $Q$ is unitary.\n",
    "\n",
    "**(d)** Since $\\Vert Q \\vec{y} \\Vert = \\Vert \\vec{y} \\Vert$ for any unitary $Q$ and $e^{Bt}$ is unitary, for the solution $\\vec{y}(t) = e^{Bt} \\vec{y}(0)$ we have\n",
    "$$\\Vert \\vec{y}(t) \\Vert^2 = \\Vert e^{Bt} \\vec{y}(0) \\Vert^2 = \\Vert \\vec{y}(0) \\Vert^2.$$\n",
    "Since $\\vec{y} = D\\vec{x} = \\begin{pmatrix} \\sqrt{k}x \\\\ \\sqrt{m}v \\end{pmatrix}$, from the above equation we have\n",
    "$$\\boxed{\\frac{1}{2} mv(t)^2 + \\frac{1}{2} kx(t)^2 = \\frac{1}{2} \\Vert \\vec{y}(t) \\Vert^2 = \\frac{1}{2} \\Vert \\vec{y}(0) \\Vert^2 = \\frac{1}{2} mv(0)^2 + \\frac{1}{2} kx(0)^2}.$$\n",
    "This shows that $\\frac{1}{2} mv^2 + \\frac{1}{2} kx^2$ is a constant as a function of $t$, i.e. the solution conserves energy."
   ]
  },
  {
   "cell_type": "markdown",
   "id": "ae091599",
   "metadata": {},
   "source": [
    "## Problem 2 (5+10)\n",
    "\n",
    "(Based on Strang, section 6.3, problem 18.)\n",
    "\n",
    "**(a)** Write five terms of the infinite series for $e^{At}$.  Take the derivative $d/dt$, and show that you have four terms of $Ae^{At}$.  \n",
    "\n",
    "Conclusion:  $\\frac{d}{dt} e^{At} = Ae^{At}$ as claimed in class, and $x(t) = e^{At}x(0)$ solves $dx/dt = Ax$.\n",
    "\n",
    "**(b)** Using the same five terms of the infinite series for $f(A) = e^A$ (no $t$), write down four terms of $f(A+dA) - f(A)$ as a *linear operator* $f'(A)[dA]$ acting on $dA$ as in Lecture 10 (i.e. drop all terms higher than first order in the \"infinitesimal\" change $dA$).\n",
    "\n",
    "$f'(A)[dA]$ is *not* simply $e^A dA$ (as it would be for scalars in 18.01) except for very special perturbations $dA$ that \\_\\_\\_\\_\\_\\_\\_\\_\\_\\_\\_\\_\\_\\_."
   ]
  },
  {
   "cell_type": "markdown",
   "id": "22273d1e",
   "metadata": {},
   "source": [
    "### Solution\n",
    "\n",
    "**(a)** Note that $e^{At} = I + At + \\frac{(At)^2}{2} + \\frac{(At)^3}{3!} + \\frac{(At)^4}{4!} + \\dots$. Taking the derivative $d/dt$ of the first five terms, we have\n",
    "$$\\boxed{0 + A + \\frac{A^2 2t }{2} + \\frac{A^3 3t^2 }{3!} + \\frac{ A^4 4t^3}{4!} = A(I + At +\\frac{(At)^2}{2} + \\frac{(At)^3}{3!})}.$$\n",
    "This shows that we have four terms of $Ae^{At}$.\n",
    "\n",
    "**(b)** Using the first five terms of the infinite series for $f(A) = e^A = I + A + \\frac{A^2}{2} + \\frac{A^3}{3!} + \\frac{A^4}{4!} + \\dots$, four terms of $f(A+dA)-f(A)$ are\n",
    "$$(I + (A+dA) + \\frac{(A+dA)^2}{2} + \\frac{(A+dA)^3}{3!} + \\frac{(A+dA)^4}{4!}) - (I + A + \\frac{A^2}{2} + \\frac{A^3}{3!} + \\frac{A^4}{4!}) \\\\\n",
    "\\approx dA+\\frac{A(dA)+(dA) A}{2} + \\frac{A^2 (dA) + A (dA) A+ (dA) A^2}{6} + \\frac{A^3(dA) + A^2 (dA) A + A (dA) A^2 + (dA) A^3}{24},$$\n",
    "where all terms higher than first order in $dA$ are dropped. Therefore, we have\n",
    "$$\\boxed{f'(A)[dA] = dA+\\frac{A(dA)+(dA) A}{2} + \\frac{A^2 (dA) + A (dA) A+ (dA) A^2}{6} + \\frac{A^3(dA) + A^2 (dA) A + A (dA) A^2 + (dA) A^3}{24}}.$$\n",
    "\n",
    "$f'(A)[dA]$ is *not* simply $e^A dA$ except for very special perturbations $dA$ that satisfy $\\boxed{A (dA) = (dA) A}$. To see this, note that if the condition is satisifed, we have\n",
    "$$dA+\\frac{A(dA)+(dA) A}{2} + \\frac{A^2 (dA) + A (dA) A+ (dA) A^2}{6} + \\frac{A^3(dA) + A^2 (dA) A + A (dA) A^2 + (dA) A^3}{24} \\\\\n",
    "= dA+\\frac{2A(dA)}{2} + \\frac{3A^2 (dA)}{6} + \\frac{4A^3(dA)}{24} = (I + A + \\frac{A^2}{2} + \\frac{A^3}{3!}) dA,$$\n",
    "which suggests that $f'(A)[dA] = e^A dA$."
   ]
  },
  {
   "cell_type": "markdown",
   "id": "0c4c58f8",
   "metadata": {},
   "source": [
    "## Problem 3 (5+5+5+5+5)\n",
    "\n",
    "**(a)** Write down two familiar functions that solve the equation $d^2 y /dt^2 = -9y$.  What is a solution $y(t)$ that starts with $y(0)=3$ and $y'(0)=0$?\n",
    "\n",
    "**(b)** Find (by hand) the eigenvalues $\\lambda_1$ and $\\lambda_2$ and corresponding eigenvectors $x_1$ and $x_2$ of $$A = \\begin{pmatrix}\n",
    "1 & -5\\\\\n",
    "10 & -14\\\\\n",
    "\\end{pmatrix} .$$\n",
    "\n",
    "**(c)** Consider the system of ODEs $\\frac{d^2x}{dt^2} = Ax$ (note 2nd derivative!) with the $A$ from part (b).  If $x(t) = c_1(t) x_1 + c_2(t) x_2$, what equations do $c_1(t)$ and $c_2(t)$ satisfy, and hence what solutions $c_1(t)$ and $c_2(t)$ are possible?   (See part (a).)\n",
    "\n",
    "**(d)** For the ODE of part (c), solve for $x(t)$ given the initial conditions $x(0) = (2,3)$ and $x'(0) = (1,4)$.\n",
    "\n",
    "**(e)** Alternatively, if we let $y$ be the 4-component vector $y = (x, dx/dt)$, then $dy/dt = By$ for $B = \\_\\_\\_\\_$.  Since this must ultimately give the same solutions $x(t)$ as part (c), what must be the eigenvalues of $B$?"
   ]
  },
  {
   "cell_type": "markdown",
   "id": "6cc4498f",
   "metadata": {},
   "source": [
    "### Solution\n",
    "\n",
    "**(a)** It can be observed that two functions that solve the equation are $\\boxed{\\cos(3t)}$ and $\\boxed{\\sin(3t)}$, or any linear combination thereof.  (You could also use $e^{\\pm i 3t} = \\cos(3t)\\pm i\\sin(3t)$, but this is redundant, just a linear combination of sines and cosines.) Therefore, the general solution is \n",
    "$$ y(t) = a \\cos(3t) + b \\sin(3t).$$\n",
    "Since $y(0) = 3$, we have $a = 3$.\n",
    "Since $y'(0) = 0$, we have $3b = 0 \\Longleftrightarrow b = 0$.\n",
    "Therefore, we have\n",
    "$$ \\boxed{y(t) = 3\\cos(3t)}.$$\n",
    "\n",
    "**(b)** To find the eigenvalues, we consider\n",
    "$$0 = \\det(A-\\lambda I)  = \\det\\begin{pmatrix}\n",
    "1-\\lambda & -5\\\\\n",
    "10 & -14-\\lambda\\\\\n",
    "\\end{pmatrix} = (1-\\lambda)(-14-\\lambda)-(-5)(10) = \\lambda^2 + 13\\lambda + 36 = (\\lambda + 9)(\\lambda + 4).$$\n",
    "Therefore, the eigenvalues are $\\boxed{\\lambda_1 = -9}$ and $\\boxed{\\lambda_2 = -4}$.\n",
    "\n",
    "For $\\lambda_1 = -9$, we have\n",
    "$$ (A-\\lambda_1 I) x_1 = 0 \\Longleftrightarrow \\begin{pmatrix}\n",
    "10 & -5\\\\\n",
    "10 & -5\\\\\n",
    "\\end{pmatrix}x_1 = 0,$$\n",
    "from which we see that an eigenvector is $\\boxed{x_1 = \\begin{pmatrix} 1 \\\\ 2 \\end{pmatrix}}$.\n",
    "\n",
    "For $\\lambda_1 = -4$, we have\n",
    "$$ (A-\\lambda_2 I) x_2 = 0 \\Longleftrightarrow \\begin{pmatrix}\n",
    "5 & -5\\\\\n",
    "10 & -10\\\\\n",
    "\\end{pmatrix}x_2 = 0,$$\n",
    "from which we see that an eigenvector is $\\boxed{x_2 = \\begin{pmatrix} 1 \\\\ 1 \\end{pmatrix}}$.\n",
    "\n",
    "**(c)** Note that $A x_1 = -9 x_1$ and $A x_2 = -4 x_2$. Therefore, if $x(t) = c_1(t) x_1 + c_2(t) x_2$, we have\n",
    "$$Ax = A(c_1(t) x_1 + c_2(t) x_2) = -9c_1(t)x_1 -4 c_2(t) x_2.$$\n",
    "Also, we have\n",
    "$$\\frac{d^2x}{dt^2} = \\frac{d^2(c_1(t) x_1 + c_2(t) x_2)}{dt^2} = \\frac{d^2(c_1(t))}{dt^2} x_1 + \\frac{d^2(c_2(t))}{dt^2} x_2.$$ \n",
    "Therefore, for the system of ODEs $\\frac{d^2x}{dt^2} = Ax$, $c_1(t)$ and $c_2(t)$ satisfy $\\boxed{\\frac{d^2(c_1(t))}{dt^2} = -9c_1(t)}$ and $\\boxed{\\frac{d^2(c_2(t))}{dt^2} = -4c_2(t)}$. \n",
    "\n",
    "From (a), the possible solutions are\n",
    "$$\\boxed{c_1(t) = a_1 \\cos(3t) + b_1 \\sin(3t)}$$\n",
    "and \n",
    "$$\\boxed{c_2(t) = a_2 \\cos(2t) + b_2 \\sin(2t)},$$\n",
    "where $a_1, b_1, a_2, b_2$ are constants.\n",
    "\n",
    "**(d)** From the initial condition $x(0) = (2,3)$, we have $c_1(0)x_1 + c_2(0)x_2 = (2,3)$ and hence\n",
    "$$\n",
    "a_1 \\begin{pmatrix} 1 \\\\ 2 \\end{pmatrix} + a_2 \\begin{pmatrix} 1 \\\\ 1 \\end{pmatrix} =  \\begin{pmatrix} 2 \\\\ 3 \\end{pmatrix} \\Longleftrightarrow a_1 = a_2 = 1.\n",
    "$$\n",
    "\n",
    "From the initial condition $x'(0) = (1,4)$, we have $c_1'(0)x_1 + c_2'(0)x_2 = (1,4)$ and hence\n",
    "$$\n",
    "3b_1 \\begin{pmatrix} 1 \\\\ 2 \\end{pmatrix} + 2b_2 \\begin{pmatrix} 1 \\\\ 1 \\end{pmatrix} =  \\begin{pmatrix} 1 \\\\ 4 \\end{pmatrix} \\Longleftrightarrow b_1 = b_2 = \\frac{1}{2}.\n",
    "$$\n",
    "\n",
    "Therefore, the solution is\n",
    "$$\\boxed{x(t) = (\\cos(3t) + \\frac{\\sin(3t)}{2}) \\begin{pmatrix} 1 \\\\ 2 \\end{pmatrix} + (\\cos(2t) + \\frac{\\sin(2t)}{2}) \\begin{pmatrix} 1 \\\\ 1 \\end{pmatrix} = \\begin{pmatrix} \\cos(3t) + \\frac{\\sin(3t)}{2} +\\cos(2t) + \\frac{\\sin(2t)}{2} \\\\ 2\\cos(3t) + \\sin(3t) + \\cos(2t) + \\frac{\\sin(2t)}{2} \\end{pmatrix}} .$$\n",
    "\n",
    "**(e)** If $y = (x, dx/dt)$, then \n",
    "$$\n",
    "\\frac{dy}{dt} = \\begin{pmatrix} \\frac{dx}{dt} \\\\ \\frac{d^2x}{dt^2} \\end{pmatrix} = \\begin{pmatrix} \\frac{dx}{dt} \\\\ Ax \\end{pmatrix} = \\begin{pmatrix} 0 & I \\\\ A & 0 \\end{pmatrix} \\begin{pmatrix} x \\\\ \\frac{dx}{dt} \\end{pmatrix} = \\begin{pmatrix} 0 & 0 & 1 & 0 \\\\ 0 & 0 & 0 & 1 \\\\ 1 & -5 & 0 & 0 \\\\ 10 & -14 & 0 & 0 \\end{pmatrix}\\begin{pmatrix} x \\\\ \\frac{dx}{dt} \\end{pmatrix} = \\begin{pmatrix} 0 & 0 & 1 & 0 \\\\ 0 & 0 & 0 & 1 \\\\ 1 & -5 & 0 & 0 \\\\ 10 & -14 & 0 & 0 \\end{pmatrix}y.$$ \n",
    "Therefore, we have $\\boxed{B = \\begin{pmatrix} 0 & 0 & 1 & 0 \\\\ 0 & 0 & 0 & 1 \\\\ 1 & -5 & 0 & 0 \\\\ 10 & -14 & 0 & 0 \\end{pmatrix}}$.\n",
    "\n",
    "Since this must ultimately give the same solutions $x(t)$ as part (c), but has solutions $y(t)=e^{Bt} y(0)$, we see that the eigenvalues of $B$ must be **purely imaginary** and consist of the **frequencies** of the problem, i.e. ± the square roots of the eigenvalues of $A$, i.e. $$\\boxed{\\pm 3i \\mbox{ and } \\pm 2i}.$$"
   ]
  },
  {
   "cell_type": "markdown",
   "id": "d920ed64",
   "metadata": {},
   "source": [
    "\n",
    "## Problem 4 (8+8)\n",
    "\n",
    "In chemistry, the [stoichiometry matrix](https://en.wikipedia.org/wiki/Stoichiometry#Stoichiometry_matrix) is often used to describe a set of $m$ reactions among $n$ different chemical \"species\" (e.g. H₂O, C₈H₁₀N₄O₂, and so on).\n",
    "\n",
    "For example, consider the following 3 (fictitious) chemical reactions among 4 species, labeled $x_1, x_2, x_3, x_4$:\n",
    "\n",
    "$$\n",
    "x_1 + 2x_2 \\longleftrightarrow 3 x_2 + 2x_4 \\\\\n",
    "2x_2 + 4x_3 \\longleftrightarrow x_1 + x_4 \\\\\n",
    "x_1 + 4x_3 \\longleftrightarrow 5x_4\n",
    "$$\n",
    "\n",
    "which would be represented by the stoichiometry matrix\n",
    "\n",
    "$$\n",
    "S = \\begin{pmatrix} -1 & 3-2 & 0 & 2 \\\\\n",
    "1 & -2 & -4 & 1 \\\\\n",
    "-1 & 0 & -4 & 5 \\end{pmatrix}\n",
    "$$\n",
    "\n",
    "whose rows are the reactions and whose columns are the species.  (Some authors use the transpose of this matrix instead.)\n",
    "\n",
    "If we use a vector $\\vec{x} \\in \\mathbb{R}^4$ to represent the *concentrations* of each of these four species, and a vector $\\vec{r} \\in \\mathbb{R}^3$ to represent the *rates* of each reaction, then the rate of change of the concentrations is given by the system of ordinary differential equations (ODEs):\n",
    "\n",
    "$$\n",
    "\\frac{d\\vec{x}}{dt} = S^T \\vec{r}\n",
    "$$\n",
    "\n",
    "(where the rates $\\vec{r}$ are *not* generally constant: they may depend on the concentrations $\\vec{x}$ in a complicated way … so you *can't* solve this just by multiplying the right-hand side by $t$).\n",
    "\n",
    "**(a)** Describe (find a basis for) *all* possible reaction rates $\\vec{r}$ for which $\\frac{d\\vec{x}}{dt} = 0$ (the system is in *steady state*).\n",
    "\n",
    "**(b)** Certain linear combinations of the concentrations are *conserved*: there are some (time-independent) vectors $\\vec{v} \\in \\mathbb{R}^4$ for which $\\frac{d(\\vec{v}^T \\vec{x})}{dt} = 0$ for *all* possible rate vectors $\\vec{r}$.   If $\\vec{v}$ doesn't depend on $t$, then $\\frac{d(\\vec{v}^T \\vec{x})}{dt}$ is \\_\\_\\_\\_\\_\\_\\_\\_ times $\\frac{d\\vec{x}}{dt}$. These vectors $\\vec{v}$ all lie within the \\_\\_\\_-dimensional \\_\\_\\_\\_\\_\\_\\_\\_ space of $S$.  Why?"
   ]
  },
  {
   "cell_type": "markdown",
   "id": "c94dda52",
   "metadata": {},
   "source": [
    "## Solution\n",
    "\n",
    "**(a)** The system is in steady state if $\\frac{d\\vec{x}}{dt} = S^T \\vec{r} = 0$. This occurs if and only if $\\vec{r}$ is in the **left nullspace** of $S$: $\\boxed{\\vec{r}\\in N(S^T)}$. To find a basis for $N(S^T)$, we apply Gaussian elimination:\n",
    "\\begin{align}\n",
    "S^T = \\begin{pmatrix} -1 & 1 & -1\\\\ 1 & -2 & 0 \\\\0 & -4 & -4 \\\\ 2 & 1& 5 \\end{pmatrix}\n",
    "\\rightarrow \\begin{pmatrix} -1 & 1 & -1\\\\ 0 & -1 & -1 \\\\0 & -4 & -4 \\\\ 0 & 3 & 3 \\end{pmatrix}\n",
    "\\rightarrow \\begin{pmatrix} 1 & -1 & 1\\\\ 0 & -1 & -1 \\\\0 & 0 & 0 \\\\ 0 & 0 & 0 \\end{pmatrix}\n",
    "\\end{align}\n",
    "\n",
    "We see that $S^T$ has two pivot columns, and one free column. We can deduce that $\\mathrm{rank}(S)=\\mathrm{rank}(S^T)=2$. Since $S^T$ has three columns, it will have a one dimensional nullspace. We can then find the special solution of $S^Tx = 0$, which is $x= \\begin{pmatrix} -2 \\\\ -1 \\\\ 1 \\end{pmatrix}$. \n",
    "\n",
    "Therefore the reaction rates for which $\\vec{r}$ for which $\\frac{d\\vec{x}}{dt} = 0$ are of the form\n",
    "\\begin{align}\n",
    "\\boxed{\\vec{r} = r_0\\begin{pmatrix} -2 \\\\ -1 \\\\ 1 \\end{pmatrix}}\n",
    "\\end{align}\n",
    "for all scalars $r_0\\in\\mathbb{R}$.\n",
    "\n",
    "**(b)** We want to find $\\vec{v}$ independent of time, for which $\\frac{d(\\vec{v}^T \\vec{x})}{dt} = 0$ for *all* possible rate vectors $\\vec{r}$. If $\\vec{v}$ doesn't depend on $t$, then \n",
    "\\begin{align}\n",
    "\\frac{d(\\vec{v}^T \\vec{x})}{dt} = \\boxed{\\vec{v}^T}\\frac{d\\vec{x}}{dt} = \\vec{v}^T S^T \\vec{r} = 0.\n",
    "\\end{align}\n",
    "We seek $\\vec{v}$ for which this is true for *all* $\\vec{r}$, and so $\\vec{v}^T S^T = 0 \\implies S\\vec{v} = 0$. Therefore, the vectors $\\vec{v}$ all lie within the $4-2 = \\boxed{2}$-dimensional **nullspace** of $S$. \n",
    "\n",
    "Although you were **not required to do so,** we can find a basis for such $\\vec{v}$ by finding the nullspace of $S$:\n",
    "\\begin{align}\n",
    "S = \\begin{pmatrix} -1 & 1 & 0 & 2 \\\\ 1 & -2 & -4 & 1 \\\\ -1 & 0 & -4 & 5 \\end{pmatrix}\n",
    "\\rightarrow \\begin{pmatrix} -1 & 1 & 0 & 2 \\\\ 0 & -1 & -4 & 3 \\\\  0 & -1 & -4 & 3  \\end{pmatrix}\n",
    "\\rightarrow \\begin{pmatrix} 1 & -1 & 0 & -2 \\\\ 0 & 1 & 4 & -3 \\\\  0 & 0 & 0 & 0  \\end{pmatrix}\n",
    "\\rightarrow \\begin{pmatrix} 1 & 0 & 4 & -5 \\\\ 0 & 1 & 4 & -3 \\\\  0 & 0 & 0 & 0  \\end{pmatrix}\n",
    "\\end{align}\n",
    "\n",
    "We can then calculate the special solutions of $Sx = 0$, which are \n",
    "\\begin{align}\n",
    "\\begin{pmatrix} -4 \\\\ -4 \\\\ 1 \\\\ 0 \\end{pmatrix} \\;\\; \\text{and} \\;\\; \\begin{pmatrix} 5 \\\\ 3 \\\\ 0 \\\\ 1 \\end{pmatrix}\n",
    "\\end{align}\n",
    "\n",
    "We conclude that $\\frac{d(\\vec{v}^T \\vec{x})}{dt} = 0$ for $\\vec{v}$ of the form:\n",
    "\\begin{align}\n",
    "\\boxed{\\vec{v} = c_1 \\begin{pmatrix} -4 \\\\ -4 \\\\ 1 \\\\ 0 \\end{pmatrix} + c_2\\begin{pmatrix} 5 \\\\ 3 \\\\ 0 \\\\ 1 \\end{pmatrix}}\n",
    "\\end{align}"
   ]
  }
 ],
 "metadata": {
  "kernelspec": {
   "display_name": "Julia 1.7.2",
   "language": "julia",
   "name": "julia-1.7"
  },
  "language_info": {
   "file_extension": ".jl",
   "mimetype": "application/julia",
   "name": "julia",
   "version": "1.7.2"
  }
 },
 "nbformat": 4,
 "nbformat_minor": 5
}
